code/k256/Hacl.Impl.K256.Point.fsti
@@ -158,7 +158,7 @@ val point_negate_conditional_vartime: p:point -> is_negate:bool -> Stack unit
       (if is_negate then S.point_negate (point_eval h0 p) else point_eval h0 p))
 
 
-val point_eq (p q:point) : Stack bool
+val point_eq_vartime (p q:point) : Stack bool
   (requires fun h ->
     live h p /\ live h q /\ eq_or_disjoint p q /\
     point_inv h p /\ point_inv h q)
